

Derivations

Erik An

<2025-12-06 Sat>

Contents

1	Given formulas to use	2
2	Mean Square Error	2

1 Given formulas to use

$$estimatePrice(mileage) = \theta_0 + (\theta_1 \times mileage)$$

$$tmp\theta_0 = learningRate \times \frac{1}{m} \times \sum_{i=0}^{m-1} (estimatePrice(mileage[i]) - price[i])$$

$$tmp\theta_1 = learningRate \times \frac{1}{m} \times \sum_{i=0}^{m-1} (estimatePrice(mileage[i]) - price[i]) \times mileage[i]$$

2 Mean Square Error

$$MSE = \frac{1}{n} \times \sum_{i=1}^n (Y_i - \hat{Y}_i)^2$$

where:

n amount of observation quantities

Y_i observed quantities

\hat{Y}_i predicted quantities

Hence,

$$MSE' = \frac{2}{n} \times \sum_{i=1}^n (Y_i - \hat{Y}_i)$$

which looks familiar, since it basically is the given formulas.